spc/HoareDef.v
@@ -559,6 +559,10 @@ Section SMOD.
   Definition to_tgt (stb: Sk.t -> gname -> option fspec) (md: t): Mod.t :=
     transl (fun sk mn => fun_to_tgt mn (stb sk)) (fun ms => Any.pair ms.(SModSem.initial_st) ms.(SModSem.initial_mr)↑) md.
 
+  Definition get_stb (mds: list t): Sk.t -> alist gname fspec :=
+    fun sk => map map_snd fsb_fspec (flat_map (fun md => (md.(get_modsem) sk).(SModSem.fnsems)) mds).
+
+
   (* Definition transl (tr: SModSem.t -> ModSem.t) (md: t): Mod.t := {| *)
   (*   Mod.get_modsem := (SModSem.transl tr) ∘ md.(get_modsem); *)
   (*   Mod.sk := md.(sk); *)
